Logic/Predicate/Semantics.lean
@@ -2,107 +2,90 @@ import Logic.Predicate.Term
 
 universe u u₁ u₂ v v₁ v₂ w w₁ w₂
 
-variable
-  {L : Language.{u}} {L₁ : Language.{u₁}} {L₂ : Language.{u₂}}
-  {μ : Type v} {μ₁ : Type v₁} {μ₂ : Type v₂}
-
 namespace FirstOrder
-variable (L)
 
-@[ext] class Structure (M : Type w) where
-  func : {k : ℕ} → L.func k → (Fin k → M) → M
-  rel  : {k : ℕ} → L.rel k → (Fin k → M) → Prop
+variable
+  {L : ℕ → Type u} {L₁ : ℕ → Type u₁} {L₂ : ℕ → Type u₂}
+  {μ : Type v} {μ₁ : Type v₁} {μ₂ : Type v₂}
+  {n n₁ n₂ n₃ : ℕ}
 
-@[ext] structure Structure.Hom (M₁ : Type w₁) (M₂ : Type w₂) [s₁ : Structure L M₁] [s₂ : Structure L M₂] where
+-- Structure of Term
+@[ext] class TStructure (L : ℕ → Type u) (M : Type w) where
+  func : ⦃k : ℕ⦄ → L k → (Fin k → M) → M
+
+namespace TStructure
+
+instance [Inhabited M] : Inhabited (TStructure L M) := ⟨{ func := fun _ _ => default }⟩
+
+structure Hom (L : ℕ → Type u) (M₁ : Type w₁) (M₂ : Type w₂) [s₁ : TStructure L M₁] [s₂ : TStructure L M₂] where
   toFun : M₁ → M₂
-  toFun_func' : ∀ {k} (f : L.func k) (v : Fin k → M₁), toFun (s₁.func f v) = s₂.func f (fun i => toFun (v i))
-  toFun_rel' : ∀ {k} (r : L.rel k) (v : Fin k → M₁), s₁.rel r v ↔ s₂.rel r (fun i => toFun (v i))
+  toFun_func' : ∀ {k} (f : L k) (v : Fin k → M₁), toFun (s₁.func f v) = s₂.func f (fun i => toFun (v i))
 
-notation:25 M " →ₛ[" L "] " M' => Structure.Hom L M M'
-
-instance (M : Type w) (M' : Type w') [Structure L M] [Structure L M'] :
-  CoeFun (M →ₛ[L] M') (fun _ => M → M') := ⟨fun f => f.toFun⟩
-
-class SubStructure (M₁ : Type w₁) (M₂ : Type w₂) [Structure L M₁] [Structure L M₂] where
-  inclusion : M₁ →ₛ[L] M₂
-  inclusion_inj : Function.Injective inclusion.toFun
-
-notation:25 M₁ " ⊆ₛ[" L "] " M₂ => SubStructure L M₁ M₂
-
-@[ext] structure Structure.ClosedSubset (M : Type w) [s : Structure L M] where
-  domain : Set M
-  domain_closed : ∀ {k} (f : L.func k) {v : Fin k → M}, (∀ i, v i ∈ domain) → s.func f v ∈ domain
-
-instance (M : Type w) [Structure L M] : SetLike (Structure.ClosedSubset L M) M := ⟨Structure.ClosedSubset.domain, Structure.ClosedSubset.ext⟩
-
-end FirstOrder
-
-namespace Language
+notation:25 M " →ᴱₛ[" L "] " M' => Hom L M M'
 
 namespace Hom
 
-open FirstOrder
+variable {M : Type w} {M' : Type w'} [TStructure L M] [TStructure L M']
 
-def onStructure (Φ : L₁ →ᵥ L₂) {M : Type w} (S : Structure L₂ M) : Structure L₁ M where
-  func := fun f => S.func (Φ.onFunc f)
-  rel := fun r => S.rel (Φ.onRel r)
+instance : FunLike (M →ᴱₛ[L] M') M (fun _ => M') where
+  coe := TStructure.Hom.toFun
+  coe_injective' := fun φ ψ h => by rcases φ; rcases ψ; simp; exact h
 
-instance subLanguageStructure {pf : ∀ k, Language.func L k → Prop} {pr : ∀ k, L.rel k → Prop}
-  {M : Type w} (s : Structure L M) : Structure (subLanguage L pf pr) M :=
-  onStructure (ofSubLanguage L) s
+instance : CoeFun (M →ᴱₛ[L] M') (fun _ => M → M') := ⟨fun f => f.toFun⟩
 
-noncomputable def extendStructure (Φ : L₁ →ᵥ L₂) {M : Type w} [Inhabited M] (s : Structure L₁ M) : Structure L₂ M where
-  func := fun {k} f₂ v => Classical.epsilon (fun y => ∃ f₁ : L₁.func k, Φ.onFunc f₁ = f₂ ∧ y = s.func f₁ v)
-  rel  := fun {k} r₂ v => ∃ r₁ : L₁.rel k, Φ.onRel r₁ = r₂ ∧ s.rel r₁ v
+@[ext] lemma ext (φ ψ : M →ᴱₛ[L] M') (h : ∀ x, φ x = ψ x) : φ = ψ := FunLike.ext φ ψ h
 
 end Hom
-end Language
 
-namespace FirstOrder
+end TStructure
 
-namespace Structure
+class SubTStructure (L : ℕ → Type u) (M₁ : Type w₁) (M₂ : Type w₂) [TStructure L M₁] [TStructure L M₂] where
+  inclusion : M₁ →ᴱₛ[L] M₂
+  inclusion_inj : Function.Injective inclusion.toFun
 
-instance [Inhabited M] : Inhabited (Structure L M) :=
-⟨{ func := fun _ _ => default, rel := fun _ _ => True }⟩
+notation:25 M₁ " ⊆ᴱₛ[" L "] " M₂ => SubTStructure L M₁ M₂
 
-variable (Φ : L₁ →ᵥ L₂) {M : Type w} (s₂ : Structure L₂ M)
+@[ext] structure TStructure.ClosedSubset (L : ℕ → Type u) (M : Type w) [s : TStructure L M] where
+  domain : Set M
+  domain_closed : ∀ {k} (f : L k) {v : Fin k → M}, (∀ i, v i ∈ domain) → s.func f v ∈ domain
 
-@[simp] lemma onStructure_func {k} {f : L₁.func k} {v : Fin k → M} :
-    (Φ.onStructure s₂).func f v = s₂.func (Φ.onFunc f) v := rfl
+instance (M : Type w) [TStructure L M] : SetLike (TStructure.ClosedSubset L M) M :=
+  ⟨TStructure.ClosedSubset.domain, TStructure.ClosedSubset.ext⟩
 
-@[simp] lemma onStructure_rel {k} {r : L₁.rel k} {v : Fin k → M} :
-    (Φ.onStructure s₂).rel r v ↔ s₂.rel (Φ.onRel r) v := of_eq rfl
+namespace TStructure
 
-variable [Inhabited M] (s₁ : Structure L₁ M)
+protected def lMap (φ : ⦃k : ℕ⦄ → L₁ k → L₂ k) {M : Type w} (S : TStructure L₂ M) : TStructure L₁ M where
+  func := fun _ f => S.func (φ f)
 
-lemma extendStructure_func
-  {k} (injf : Function.Injective (Φ.onFunc : L₁.func k → L₂.func k)) (f₁ : L₁.func k) (v : Fin k → M) :
-    (Φ.extendStructure s₁).func (Φ.onFunc f₁) v = s₁.func f₁ v := by
-  simp[Language.Hom.extendStructure]
-  have : ∃ y, ∃ f₁' : L₁.func k, Φ.onFunc f₁' = Φ.onFunc f₁ ∧ y = s₁.func f₁' v := ⟨s₁.func f₁ v, f₁, rfl, rfl⟩
+variable (φ : ⦃k : ℕ⦄ → L₁ k → L₂ k) {M : Type w} (s₂ : TStructure L₂ M)
+
+@[simp] lemma lMap_func {k} {f : L₁ k} {v : Fin k → M} :
+    (s₂.lMap φ).func f v = s₂.func (φ f) v := rfl
+
+/-
+variable [Inhabited M] (s₁ : TStructure L₁ M)
+
+lemma extendTStructure_func
+  {k} (injf : Function.Injective (φ.onFunc : L₁.func k → L₂.func k)) (f₁ : L₁.func k) (v : Fin k → M) :
+    (φ.extendTStructure s₁).func (φ.onFunc f₁) v = s₁.func f₁ v := by
+  simp[Language.Hom.extendTStructure]
+  have : ∃ y, ∃ f₁' : L₁.func k, φ.onFunc f₁' = φ.onFunc f₁ ∧ y = s₁.func f₁' v := ⟨s₁.func f₁ v, f₁, rfl, rfl⟩
   rcases Classical.epsilon_spec this with ⟨f', f'eq, h⟩
   rcases injf f'eq with rfl; exact h
 
-lemma extendStructure_rel
-  {k} (injr : Function.Injective (Φ.onRel : L₁.rel k → L₂.rel k)) (r₁ : L₁.rel k) (v : Fin k → M) :
-    (Φ.extendStructure s₁).rel (Φ.onRel r₁) v ↔ s₁.rel r₁ v := by
-  simp[Language.Hom.extendStructure]
+lemma extendTStructure_rel
+  {k} (injr : Function.Injective (φ.onRel : L₁.rel k → L₂.rel k)) (r₁ : L₁.rel k) (v : Fin k → M) :
+    (φ.extendTStructure s₁).rel (φ.onRel r₁) v ↔ s₁.rel r₁ v := by
+  simp[Language.Hom.extendTStructure]
   refine ⟨by intros h; rcases h with ⟨r₁', e, h⟩; rcases injr e; exact h, by intros h; refine ⟨r₁, rfl, h⟩⟩
 
-class Eq (L : Language.{u}) [L.Eq] (M : Type w) [s : Structure L M] where
-  eq : ∀ a b, s.rel Language.Eq.eq ![a, b] ↔ a = b
+-/
 
-attribute [simp] Eq.eq
-
-end Structure
-
-end FirstOrder
+end TStructure
 
 namespace SubTerm
 
-open FirstOrder
-
-variable {M : Type w} (s : Structure L M) {n n₁ n₂ : ℕ} (e : Fin n → M) (e₂ : Fin n₂ → M) (ε : μ → M) (ε₂ : μ₂ → M)
+variable {M : Type w} (s : TStructure L M) (e : Fin n → M) (e₁ : Fin n₁ → M) (e₂ : Fin n₂ → M) (ε : μ → M) (ε₂ : μ₂ → M)
 
 def val : SubTerm L μ n → M
   | #x       => e x
@@ -113,9 +96,9 @@ abbrev bVal (t : SubTerm L Empty n) : M := t.val s e Empty.elim
 
 variable (M) {s}
 
-abbrev val! [s : Structure L M] {n} (e : Fin n → M) (ε : μ → M) : SubTerm L μ n → M := val s e ε
+abbrev val! [s : TStructure L M] {n} (e : Fin n → M) (ε : μ → M) : SubTerm L μ n → M := val s e ε
 
-abbrev bVal! [s : Structure L M] {n} (e : Fin n → M) : SubTerm L Empty n → M := bVal s e
+abbrev bVal! [s : TStructure L M] {n} (e : Fin n → M) : SubTerm L Empty n → M := bVal s e
 
 variable {M e e₂ ε ε₂}
 
@@ -123,57 +106,58 @@ variable {M e e₂ ε ε₂}
 
 @[simp] lemma val_fvar (x) : val s e ε (&x : SubTerm L μ n) = ε x := rfl
 
-lemma val_func {k} (f : L.func k) (v) :
+lemma val_func {k} (f : L k) (v) :
     val s e ε (func f v) = s.func f (fun i => (v i).val s e ε) := rfl
 
-@[simp] lemma val_func₀ (f : L.func 0) (v) :
+@[simp] lemma val_func₀ (f : L 0) (v) :
     val s e ε (func f v) = s.func f ![] := by simp[val_func, Matrix.empty_eq]
 
-@[simp] lemma val_func₁ (f : L.func 1) (t) :
+@[simp] lemma val_func₁ (f : L 1) (t) :
     val s e ε (func f ![t]) = s.func f ![t.val s e ε] :=
   by simp[val_func]; apply of_eq; congr; funext i; cases' i using Fin.cases with i <;> simp
 
-@[simp] lemma val_func₂ (f : L.func 2) (t u) :
+@[simp] lemma val_func₂ (f : L 2) (t u) :
     val s e ε (func f ![t, u]) = s.func f ![t.val s e ε, u.val s e ε] :=
   by simp[val_func]; apply of_eq; congr; funext i; cases' i using Fin.cases with i <;> simp
 
-lemma val_bind (bound : Fin n₁ → SubTerm L μ₂ n₂) (free : μ₁ → SubTerm L μ₂ n₂) (t : SubTerm L μ₁ n₁) :
-    (bind bound free t).val s e₂ ε₂ = t.val s (val s e₂ ε₂ ∘ bound) (val s e₂ ε₂ ∘ free) :=
-  by induction t <;> simp[*, bind_func, val_func]
-
-lemma val_map (bound : Fin n₁ → Fin n₂) (free : μ₁ → μ₂) (t : SubTerm L μ₁ n₁) :
-    (map bound free t).val s e₂ ε₂ = t.val s (e₂ ∘ bound) (ε₂ ∘ free) := val_bind _ _ _
+lemma val_hom (ω : SubTerm.Hom L μ₁ n₁ μ₂ n₂) (t : SubTerm L μ₁ n₁) :
+    (ω t).val s e₂ ε₂ = t.val s (val s e₂ ε₂ ∘ ω ∘ bvar) (val s e₂ ε₂ ∘ ω ∘ fvar) :=
+  by induction t <;> simp[*, Hom.func, val_func]
 
 /-
-lemma val_subst (u : SubTerm L μ n) (t : SubTerm L μ (n + 1)) :
-    (subst u t).val s e ε = t.val s (e <: u.val s e ε) ε :=
-  by simp[subst, val_bind]; congr; exact funext $ Fin.lastCases (by simp) (by simp)
+lemma val_bind (b : Fin n₁ → SubTerm L μ₂ n₂) (e : μ₁ → SubTerm L μ₂ n₂) (t : SubTerm L μ₁ n₁) :
+    (bind b e t).val s e₂ ε₂ = t.val s (val s e₂ ε₂ ∘ b) (val s e₂ ε₂ ∘ e) :=
+  by simp[val_hom]
+
+lemma val_map (b : Fin n₁ → Fin n₂) (e : μ₁ → μ₂) (t : SubTerm L μ₁ n₁) :
+    (map b e t).val s e₂ ε₂ = t.val s (e₂ ∘ b) (ε₂ ∘ e) := by simp[val_hom]; congr
 -/
 
 lemma val_substs {n'} (w : Fin n' → SubTerm L μ n) (t : SubTerm L μ n') :
     (substs w t).val s e ε = t.val s (fun x => (w x).val s e ε) ε :=
-  by simp[substs, val_bind]; congr
+  by simp[val_hom]; congr
 
 @[simp] lemma val_bShift (a : M) (t : SubTerm L μ n) :
-    t.bShift.val s (a :> e) ε = t.val s e ε := by simp[bShift, val_map, Function.comp]
-
+    t.bShift.val s (a :> e) ε = t.val s e ε := by simp[val_hom, Function.comp]
 section Language
 
-variable (Φ : L₁ →ᵥ L₂) (e : Fin n → M) (ε : μ → M)
+variable (φ : ⦃k : ℕ⦄ → L₁ k → L₂ k) (e : Fin n → M) (ε : μ → M)
 
-lemma val_onSubTerm (s₂ : Structure L₂ M) {t : SubTerm L₁ μ n} :
-    val s₂ e ε (Φ.onSubTerm t) = val (Φ.onStructure s₂) e ε t :=
-  by induction t <;> simp[*, val!, Function.comp, val_func, Language.Hom.onSubTerm_func]
+lemma val_lMap (s₂ : TStructure L₂ M) {t : SubTerm L₁ μ n} :
+    (t.lMap φ).val s₂ e ε = t.val (s₂.lMap φ) e ε :=
+  by induction t <;> simp[*, val!, Function.comp, val_func, SubTerm.lMap_func]
 
+/-
 variable [Inhabited M]
 
-lemma val_extendStructure_onSubTerm
-    (injf : ∀ k, Function.Injective (Φ.onFunc : L₁.func k → L₂.func k))
-    (s₁ : Structure L₁ M) (t : SubTerm L₁ μ n) :
-    val (Φ.extendStructure s₁) e ε (Φ.onSubTerm t) = val s₁ e ε t := by
-  induction t <;> simp[*, Language.Hom.onSubTerm_func, val_func]
+lemma val_extendTStructure_lMap
+    (injf : ∀ k, Function.Injective (φ.onFunc : L₁.func k → L₂.func k))
+    (s₁ : TStructure L₁ M) (t : SubTerm L₁ μ n) :
+    val (φ.extendTStructure s₁) e ε (φ.lMap t) = val s₁ e ε t := by
+  induction t <;> simp[*, Language.Hom.lMap_func, val_func]
   case func k f v ih => 
-    exact Structure.extendStructure_func Φ s₁ (injf k) f (fun i => val s₁ e ε (v i))
+    exact TStructure.extendTStructure_func φ s₁ (injf k) f (fun i => val s₁ e ε (v i))
+-/
 
 end Language
 
@@ -182,83 +166,71 @@ section Syntactic
 variable (ε : ℕ → M)
 
 lemma val_shift (t : SyntacticSubTerm L n) :
-    t.shift.val s e ε = t.val s e (ε ∘ Nat.succ) := by simp[shift, val_map]
+    t.shift.val s e ε = t.val s e (ε ∘ Nat.succ) := by simp[val_hom]; congr
 
 lemma val_free (a : M) (t : SyntacticSubTerm L (n + 1)) :
     t.free.val s e (a :>ₙ ε) = t.val s (e <: a) ε :=
-  by simp[free, val_bind]; congr; exact funext $ Fin.lastCases (by simp) (by simp)
+  by simp[val_hom]; congr; exact funext $ Fin.lastCases (by simp) (by simp)
 
 lemma val_fix (a : M) (t : SyntacticSubTerm L n) :
     t.fix.val s (e <: a) ε = t.val s e (a :>ₙ ε) :=
-  by simp[fix, val_bind, Function.comp]; congr; exact funext (Nat.cases (by simp) (by simp))
+  by simp[val_hom]; congr <;> simp[Function.comp]; exact funext (Nat.cases (by simp) (by simp))
 
 end Syntactic
 
 end SubTerm
 
-namespace FirstOrder
-
-namespace Structure
+namespace TStructure
 
 namespace ClosedSubset
-variable {M : Type w} [s : Structure L M] (u : ClosedSubset L M)
 
-lemma closed {k} (f : L.func k) {v : Fin k → M} (hv : ∀ i, v i ∈ u) : s.func f v ∈ u := u.domain_closed f hv
+variable {M : Type w} [s : TStructure L M] (u : ClosedSubset L M)
 
-instance toStructure [s : Structure L M] (u : ClosedSubset L M) : Structure L u where
-  func := fun f v => ⟨s.func f (fun i => ↑(v i)), u.closed f (by simp)⟩
-  rel := fun r v => s.rel r (fun i => ↑(v i))
+lemma closed {k} (f : L k) {v : Fin k → M} (hv : ∀ i, v i ∈ u) : s.func f v ∈ u := u.domain_closed f hv
 
-lemma coe_func {k} (f : L.func k) (v : Fin k → u) : (u.toStructure.func f v : M) = s.func f (fun i => ↑(v i)) := rfl
+instance toTStructure [s : TStructure L M] (u : ClosedSubset L M) : TStructure L u where
+  func := fun k f v => ⟨s.func f (fun i => ↑(v i)), u.closed f (by simp)⟩
 
-lemma coe_rel {k} (r : L.rel k) (v : Fin k → u) : u.toStructure.rel r v ↔ s.rel r (fun i => ↑(v i)) := of_eq rfl
+lemma coe_func {k} (f : L k) (v : Fin k → u) : (u.toTStructure.func f v : M) = s.func f (fun i => ↑(v i)) := rfl
 
 end ClosedSubset
 
 namespace Hom
-variable {M₁ : Type w₁} {M₂ : Type w₂} [s₁ : Structure L M₁] [s₂ : Structure L M₂] (φ : M₁ →ₛ[L] M₂)
 
-lemma hom_func {k} (f : L.func k) (v : Fin k → M₁) :
-  φ (s₁.func f v) = s₂.func f (φ ∘ v) := φ.toFun_func' f v
+variable {M₁ : Type w₁} {M₂ : Type w₂} [s₁ : TStructure L M₁] [s₂ : TStructure L M₂] (φ : M₁ →ᴱₛ[L] M₂)
 
-lemma hom_rel {k} (r : L.rel k) (v : Fin k → M₁) :
-  s₁.rel r v ↔ s₂.rel r (φ ∘ v) := φ.toFun_rel' r v
+protected lemma func {k} (f : L k) (v : Fin k → M₁) :
+    φ (s₁.func f v) = s₂.func f (φ ∘ v) := φ.toFun_func' f v
 
-lemma hom_val (e : Fin n → M₁) (ε : μ → M₁) (t : SubTerm L μ n) :
+lemma val (e : Fin n → M₁) (ε : μ → M₁) (t : SubTerm L μ n) :
     φ (t.val s₁ e ε) = t.val s₂ (φ ∘ e) (φ ∘ ε) := by
-  induction t <;> simp[*, SubTerm.val_func, hom_func, Function.comp]
+  induction t <;> simp[*, SubTerm.val_func, Hom.func, Function.comp]
 
-def eq_of_inj [L.Eq] [s₂.Eq] (h : Function.Injective φ) : s₁.Eq where
-  eq := fun a b => by simp[φ.hom_rel, Matrix.comp_vecCons', Matrix.constant_eq_singleton, h.eq_iff, Function.comp]
-
-def inclusion [s : Structure L M] (u : ClosedSubset L M) : u →ₛ[L] M where
+def inclusion [s : TStructure L M] (u : ClosedSubset L M) : u →ᴱₛ[L] M where
   toFun := Subtype.val
   toFun_func' := by simp[ClosedSubset.coe_func]
-  toFun_rel' := by simp[ClosedSubset.coe_rel]
 
 end Hom
 
-end Structure
+end TStructure
 
-namespace SubStructure
-open Structure
+namespace SubTStructure
+open TStructure
 
 variable {M : Type w} {M₁ : Type w₁} {M₂ : Type w₂}
-  [s : Structure L M] [s₁ : Structure L M₁] [s₂ : Structure L M₂] [H : M₁ ⊆ₛ[L] M₂]
+  [s : TStructure L M] [s₁ : TStructure L M₁] [s₂ : TStructure L M₂] [H : M₁ ⊆ᴱₛ[L] M₂]
 
-def eq_of_eq [L.Eq] [s₂.Eq] : s₁.Eq := H.inclusion.eq_of_inj H.inclusion_inj
+instance closedSubset (u : ClosedSubset L M) : u ⊆ᴱₛ[L] M where
+  inclusion := TStructure.Hom.inclusion u
+  inclusion_inj := by simp[TStructure.Hom.inclusion]; exact Subtype.val_injective
 
-instance closedSubset (u : ClosedSubset L M) : u ⊆ₛ[L] M where
-  inclusion := Structure.Hom.inclusion u
-  inclusion_inj := by simp[Structure.Hom.inclusion]; exact Subtype.val_injective
-
-lemma inclusion_func {k} (f : L.func k) (v : Fin k → M₁) :
-  H.inclusion (s₁.func f v) = s₂.func f (H.inclusion ∘ v) := H.inclusion.hom_func f v
+lemma inclusion_func {k} (f : L k) (v : Fin k → M₁) :
+  H.inclusion (s₁.func f v) = s₂.func f (H.inclusion ∘ v) := H.inclusion.func f v
 
 lemma inclusion_val (e : Fin n → M₁) (ε : μ → M₁) (t : SubTerm L μ n) :
     H.inclusion (t.val s₁ e ε) = t.val s₂ (H.inclusion ∘ e) (H.inclusion ∘ ε) := 
-  H.inclusion.hom_val e ε t
-  
-end SubStructure
+  H.inclusion.val e ε t
+
+end SubTStructure
 
 end FirstOrder
