Logic/Predicate/Elab.lean
@@ -1,0 +1,222 @@
+import Logic.Predicate.Term
+
+namespace FirstOrder
+
+namespace SubTerm
+
+declare_syntax_cat subterm
+syntax:max "#" term:max : subterm
+syntax:max "&" term:max : subterm
+syntax:max "ᵀ!" term:max : subterm
+syntax num : subterm
+syntax:70 "[" term "](" subterm,* ")" : subterm
+syntax:50 subterm:50 " + " subterm:51 : subterm
+syntax:60 subterm:60 " * " subterm:61 : subterm
+syntax:65 subterm:65 " ^ " subterm:66 : subterm
+syntax:67 "exp " subterm:68 : subterm
+syntax:75 "⟨" subterm ", " subterm "⟩" : subterm
+
+syntax "(" subterm ")" : subterm
+
+syntax subterm "ᵀ⟦" subterm,* "⟧" : subterm
+syntax:80 "⤒" subterm:80 : subterm
+syntax:80 "ᵀ⇑" subterm:80 : subterm
+syntax:80 "ᵀᶠ" subterm:80 : subterm
+syntax:80 "ᵀᵇ" subterm:80 : subterm
+
+syntax "ᵀ“" subterm:0 "”" : term
+
+#check SubTerm.fix
+ 
+macro_rules
+  | `(ᵀ“ # $n:term”)                                 => `(#$n)
+  | `(ᵀ“ & $n:term ”)                                => `(&$n)
+  | `(ᵀ“ ᵀ! $t:term ”)                               => `($t)
+  | `(ᵀ“ $n:num ”)                                   => `(SubTerm.Operator.const (natLit _ $n))
+  | `(ᵀ“ [ $d:term ]( $t:subterm,* ) ”)              => do
+    let v ← t.getElems.foldrM (β := Lean.TSyntax _) (init := ← `(![])) (fun a s => `(ᵀ“$a” :> $s))
+    `(func $d $v)
+  | `(ᵀ“ $t:subterm + $u:subterm ”)                  => `(func Language.Add.add ![ᵀ“$t”, ᵀ“$u”])
+  | `(ᵀ“ $t:subterm * $u:subterm ”)                  => `(func Language.Mul.mul ![ᵀ“$t”, ᵀ“$u”])
+  | `(ᵀ“ $t:subterm ^ $u:subterm ”)                  => `(func Language.Pow.pow ![ᵀ“$t”, ᵀ“$u”])
+  | `(ᵀ“ exp $t:subterm ”)                           => `(func Language.Exp.exp ![ᵀ“$t”])
+  | `(ᵀ“ ⟨ $t:subterm, $u:subterm ⟩ ”)               => `(func Language.Pairing.pair ![ᵀ“$t”, ᵀ“$u”])
+  | `(ᵀ“ ᵀ⇑$t:subterm ”)                            => `(shift ᵀ“$t”)
+  | `(ᵀ“ $t:subterm ᵀ⟦$u:subterm,*⟧ ”)               => do
+    let v ← u.getElems.foldrM (β := Lean.TSyntax _) (init := ← `(![])) (fun a s => `(ᵀ“$a” :> $s))
+    `(substs $v ᵀ“$t”)
+  | `(ᵀ“ ⤒$t:subterm ”)                             => `(SubTerm.bShift ᵀ“$t”)
+  | `(ᵀ“ ᵀᶠ $t:subterm ”)                            => `(SubTerm.free ᵀ“$t”)
+  | `(ᵀ“ ᵀᵇ $t:subterm ”)                            => `(SubTerm.fix ᵀ“$t”)
+  | `(ᵀ“ ( $x ) ”)                                   => `(ᵀ“$x”)
+
+#check Language.Add.add
+
+#check (ᵀ“ [Language.ORingFunc.mul](&2 + &0, [Language.ORingFunc.zero]())” : SubTerm Language.ORingFunc ℕ 8)
+#check (ᵀ“ [Language.ORingFunc.mul](&2 + &0, [Language.ORingFunc.zero]())” : SubTerm Language.ORingFunc ℕ 8)
+#check ᵀ“ᵀ⇑(3 * #3 + 9)”
+#check SubTerm.func Language.Mul.mul (ᵀ“1” :> ᵀ“3” :> Matrix.vecEmpty)
+
+section delab
+open Lean PrettyPrinter Delaborator SubExpr
+
+instance : Coe NumLit (TSyntax `subterm) where
+  coe s := ⟨s.raw⟩
+
+@[app_unexpander natLit]
+def unexpsnderNatLit : Unexpander
+  | `($_ $_ $z:num) => `($z)
+  | _ => throw ()
+
+@[app_unexpander Operator.const]
+def unexpsnderOperatorConst : Unexpander
+  | `($_ $z:num) => `(ᵀ“$z”)
+  | _ => throw ()
+
+notation "lang(+)" => Language.Add.add
+notation "lang(*)" => Language.Mul.mul
+notation "lang(^)" => Language.Pow.pow
+notation "lang(exp)" => Language.Exp.exp
+notation "lang(⟨⟩)" => Language.Pairing.pair
+
+@[app_unexpander Language.Add.add]
+def unexpsnderAdd : Unexpander
+  | `($_) => `(lang(+))
+
+@[app_unexpander Language.Mul.mul]
+def unexpsnderMul : Unexpander
+  | `($_) => `(lang(*))
+
+@[app_unexpander Language.Pow.pow]
+def unexpsnderPow : Unexpander
+  | `($_) => `(lang(^))
+
+@[app_unexpander SubTerm.func]
+def unexpandFunc : Unexpander
+  | `($_ $c ![])                 => `(ᵀ“ [$c]() ”)
+  | `($_ $f ![ᵀ“ $t ”])          => `(ᵀ“ [$f]($t) ”)
+  | `($_ $f ![ᵀ“ $t ”, ᵀ“ $u ”]) => `(ᵀ“ [$f]($t, $u) ”)
+  | _                            => throw ()
+
+@[app_unexpander SubTerm.shift]
+def unexpandShift : Unexpander
+  | `($_ ᵀ“$t”) => `(ᵀ“ ᵀ⇑$t ”)
+  | _           => throw ()
+
+@[app_unexpander SubTerm.Hom.toFun]
+def unexpandHom : Unexpander
+  | `($_ shift                   ᵀ“$t”) => `(ᵀ“ ᵀ⇑$t ”)
+  | `($_ bSubst                  ᵀ“$t”) => `(ᵀ“ ⤒$t ”)
+  | `($_ ᵀ⟦→ ![]⟧               ᵀ“$t”) => `(ᵀ“ $t ᵀ⟦⟧ ”)
+  | `($_ ᵀ⟦→ ![ᵀ“$u”]⟧          ᵀ“$t”) => `(ᵀ“ $t ᵀ⟦$u⟧ ”)
+  | `($_ ᵀ⟦→ ![ᵀ“$u₁”, ᵀ“$u₂”]⟧ ᵀ“$t”) => `(ᵀ“ $t ᵀ⟦$u₁, $u₂⟧ ”)
+  | _                                   => throw ()
+
+@[app_unexpander SubTerm.bShift]
+def unexpandBShift : Unexpander
+  | `($_ ᵀ“$t”) => `(ᵀ“ ⤒$t ”)
+  | _           => throw ()
+
+@[app_unexpander SubTerm.substs]
+def unexpandSubsts : Unexpander
+  | `($_ ![]               ᵀ“$t”) => `(ᵀ“ $t ᵀ⟦⟧ ”)
+  | `($_ ![ᵀ“$u”]          ᵀ“$t”) => `(ᵀ“ $t ᵀ⟦$u⟧ ”)
+  | `($_ ![ᵀ“$u₁”, ᵀ“$u₂”] ᵀ“$t”) => `(ᵀ“ $t ᵀ⟦$u₁, $u₂⟧ ”)
+  | _                             => throw ()
+
+@[app_unexpander SubTerm.free]
+def unexpandFree : Unexpander
+  | `($_ ᵀ“$t”) => `(ᵀ“ ᵀᶠ $t ”)
+  | _           => throw ()
+
+@[app_unexpander SubTerm.fix]
+def unexpandFix : Unexpander
+  | `($_ ᵀ“$t”) => `(ᵀ“ ᵀᵇ $t ”)
+  | _           => throw ()
+
+@[app_unexpander SubTerm.func]
+def unexpandFuncArith : Unexpander
+  | `($_ lang(exp) ![ᵀ“$t:subterm”]) => `(ᵀ“ exp $t ”)
+  | `($_ lang(exp) ![#$x:term])      => `(ᵀ“ exp #$x ”)
+  | `($_ lang(exp) ![&$x:term])      => `(ᵀ“ exp &$x ”)
+  | `($_ lang(exp) ![$t])            => `(ᵀ“ exp ᵀ!$t ”)
+
+  | `($_ lang(+) ![ᵀ“$t:subterm”, ᵀ“$u:subterm”]) => `(ᵀ“ ($t + $u) ”)
+  | `($_ lang(+) ![ᵀ“$t:subterm”, #$x:term     ]) => `(ᵀ“ ($t + #$x) ”)
+  | `($_ lang(+) ![ᵀ“$t:subterm”, &$x:term     ]) => `(ᵀ“ ($t + &$x) ”)
+  | `($_ lang(+) ![ᵀ“$t:subterm”, $u           ]) => `(ᵀ“ ($t + ᵀ!$u) ”)
+  | `($_ lang(+) ![#$x:term,      ᵀ“$u:subterm”]) => `(ᵀ“ (#$x + $u) ”)
+  | `($_ lang(+) ![#$x:term,      #$y:term     ]) => `(ᵀ“ (#$x + #$y) ”)
+  | `($_ lang(+) ![#$x:term,      &$y:term     ]) => `(ᵀ“ (#$x + &$y) ”)
+  | `($_ lang(+) ![#$x:term,      $u           ]) => `(ᵀ“ (#$x + ᵀ!$u) ”)
+  | `($_ lang(+) ![&$x:term,      ᵀ“$u:subterm”]) => `(ᵀ“ (&$x + $u) ”)
+  | `($_ lang(+) ![&$x:term,      #$y:term     ]) => `(ᵀ“ (&$x + #$y) ”)
+  | `($_ lang(+) ![&$x:term,      &$y:term     ]) => `(ᵀ“ (&$x + &$y) ”)
+  | `($_ lang(+) ![&$x:term,      $u           ]) => `(ᵀ“ (&$x + ᵀ!$u) ”)
+  | `($_ lang(+) ![$t,            ᵀ“$u:subterm”]) => `(ᵀ“ (ᵀ!$t + $u) ”)
+  | `($_ lang(+) ![$t,            #$y:term     ]) => `(ᵀ“ (ᵀ!$t + #$y) ”)
+  | `($_ lang(+) ![$t,            &$y:term     ]) => `(ᵀ“ (ᵀ!$t + &$y) ”)
+  | `($_ lang(+) ![$t,            $u           ]) => `(ᵀ“ (ᵀ!$t + ᵀ!$u) ”)
+
+  | `($_ lang(*) ![ᵀ“$t:subterm”, ᵀ“$u:subterm”]) => `(ᵀ“ ($t * $u) ”)
+  | `($_ lang(*) ![ᵀ“$t:subterm”, #$x:term     ]) => `(ᵀ“ ($t * #$x) ”)
+  | `($_ lang(*) ![ᵀ“$t:subterm”, &$x:term     ]) => `(ᵀ“ ($t * &$x) ”)
+  | `($_ lang(*) ![ᵀ“$t:subterm”, $u           ]) => `(ᵀ“ ($t * ᵀ!$u) ”)
+  | `($_ lang(*) ![#$x:term,      ᵀ“$u:subterm”]) => `(ᵀ“ (#$x * $u) ”)
+  | `($_ lang(*) ![#$x:term,      #$y:term     ]) => `(ᵀ“ (#$x * #$y) ”)
+  | `($_ lang(*) ![#$x:term,      &$y:term     ]) => `(ᵀ“ (#$x * &$y) ”)
+  | `($_ lang(*) ![#$x:term,      $u           ]) => `(ᵀ“ (#$x * ᵀ!$u) ”)
+  | `($_ lang(*) ![&$x:term,      ᵀ“$u:subterm”]) => `(ᵀ“ (&$x * $u) ”)
+  | `($_ lang(*) ![&$x:term,      #$y:term     ]) => `(ᵀ“ (&$x * #$y) ”)
+  | `($_ lang(*) ![&$x:term,      &$y:term     ]) => `(ᵀ“ (&$x * &$y) ”)
+  | `($_ lang(*) ![&$x:term,      $u           ]) => `(ᵀ“ (&$x * ᵀ!$u) ”)
+  | `($_ lang(*) ![$t,            ᵀ“$u:subterm”]) => `(ᵀ“ (ᵀ!$t * $u) ”)
+  | `($_ lang(*) ![$t,            #$y:term     ]) => `(ᵀ“ (ᵀ!$t * #$y) ”)
+  | `($_ lang(*) ![$t,            &$y:term     ]) => `(ᵀ“ (ᵀ!$t * &$y) ”)
+  | `($_ lang(*) ![$t,            $u           ]) => `(ᵀ“ (ᵀ!$t * ᵀ!$u) ”)
+
+  | `($_ lang(^) ![ᵀ“$t:subterm”, ᵀ“$u:subterm”]) => `(ᵀ“ ($t ^ $u) ”)
+  | `($_ lang(^) ![ᵀ“$t:subterm”, #$x:term     ]) => `(ᵀ“ ($t ^ #$x) ”)
+  | `($_ lang(^) ![ᵀ“$t:subterm”, &$x:term     ]) => `(ᵀ“ ($t ^ &$x) ”)
+  | `($_ lang(^) ![ᵀ“$t:subterm”, $u           ]) => `(ᵀ“ ($t ^ ᵀ!$u) ”)
+  | `($_ lang(^) ![#$x:term,      ᵀ“$u:subterm”]) => `(ᵀ“ (#$x ^ $u) ”)
+  | `($_ lang(^) ![#$x:term,      #$y:term     ]) => `(ᵀ“ (#$x ^ #$y) ”)
+  | `($_ lang(^) ![#$x:term,      &$y:term     ]) => `(ᵀ“ (#$x ^ &$y) ”)
+  | `($_ lang(^) ![#$x:term,      $u           ]) => `(ᵀ“ (#$x ^ ᵀ!$u) ”)
+  | `($_ lang(^) ![&$x:term,      ᵀ“$u:subterm”]) => `(ᵀ“ (&$x ^ $u) ”)
+  | `($_ lang(^) ![&$x:term,      #$y:term     ]) => `(ᵀ“ (&$x ^ #$y) ”)
+  | `($_ lang(^) ![&$x:term,      &$y:term     ]) => `(ᵀ“ (&$x ^ &$y) ”)
+  | `($_ lang(^) ![&$x:term,      $u           ]) => `(ᵀ“ (&$x ^ ᵀ!$u) ”)
+  | `($_ lang(^) ![$t,            ᵀ“$u:subterm”]) => `(ᵀ“ (ᵀ!$t ^ $u) ”)
+  | `($_ lang(^) ![$t,            #$y:term     ]) => `(ᵀ“ (ᵀ!$t ^ #$y) ”)
+  | `($_ lang(^) ![$t,            &$y:term     ]) => `(ᵀ“ (ᵀ!$t ^ &$y) ”)
+  | `($_ lang(^) ![$t,            $u           ]) => `(ᵀ“ (ᵀ!$t ^ ᵀ!$u) ”)
+
+  | `($_ lang(⟨⟩) ![ᵀ“$t:subterm”, ᵀ“$u:subterm”]) => `(ᵀ“ ⟨$t, $u  ⟩ ”)
+  | `($_ lang(⟨⟩) ![ᵀ“$t:subterm”, #$x:term     ]) => `(ᵀ“ ⟨$t, #$x ⟩ ”)
+  | `($_ lang(⟨⟩) ![ᵀ“$t:subterm”, &$x:term     ]) => `(ᵀ“ ⟨$t, &$x ⟩ ”)
+  | `($_ lang(⟨⟩) ![ᵀ“$t:subterm”, $u           ]) => `(ᵀ“ ⟨$t, ᵀ!$u⟩ ”)
+  | `($_ lang(⟨⟩) ![#$x:term,      ᵀ“$u:subterm”]) => `(ᵀ“ ⟨#$x, $u  ⟩ ”)
+  | `($_ lang(⟨⟩) ![#$x:term,      #$y:term     ]) => `(ᵀ“ ⟨#$x, #$y ⟩ ”)
+  | `($_ lang(⟨⟩) ![#$x:term,      &$y:term     ]) => `(ᵀ“ ⟨#$x, &$y ⟩ ”)
+  | `($_ lang(⟨⟩) ![#$x:term,      $u           ]) => `(ᵀ“ ⟨#$x, ᵀ!$u⟩ ”)
+  | `($_ lang(⟨⟩) ![&$x:term,      ᵀ“$u:subterm”]) => `(ᵀ“ ⟨&$x, $u  ⟩ ”)
+  | `($_ lang(⟨⟩) ![&$x:term,      #$y:term     ]) => `(ᵀ“ ⟨&$x, #$y ⟩ ”)
+  | `($_ lang(⟨⟩) ![&$x:term,      &$y:term     ]) => `(ᵀ“ ⟨&$x, &$y ⟩ ”)
+  | `($_ lang(⟨⟩) ![&$x:term,      $u           ]) => `(ᵀ“ ⟨&$x, ᵀ!$u⟩ ”)
+  | `($_ lang(⟨⟩) ![$t,            ᵀ“$u:subterm”]) => `(ᵀ“ ⟨ᵀ!$t, $u  ⟩ ”)
+  | `($_ lang(⟨⟩) ![$t,            #$y:term     ]) => `(ᵀ“ ⟨ᵀ!$t, #$y ⟩ ”)
+  | `($_ lang(⟨⟩) ![$t,            &$y:term     ]) => `(ᵀ“ ⟨ᵀ!$t, &$y ⟩ ”)
+  | `($_ lang(⟨⟩) ![$t,            $u           ]) => `(ᵀ“ ⟨ᵀ!$t, ᵀ!$u⟩ ”)
+  | _                                             => throw ()
+
+#check natLit Language.ORingFunc 99
+#check (ᵀ“1 + 8” : SubTerm Language.ORingFunc ℕ 8)
+#check (SubTerm.func Language.Mul.mul (ᵀ“1” :> ᵀ“3” :> Matrix.vecEmpty) : SubTerm Language.ORingFunc ℕ 8)
+#check ᵀ“3 + 8 * exp &6 + 2 *#0”
+#check SubTerm.substs ![&0, &5] ᵀ“(3 * #3 + 9)”
+end delab
+
+end SubTerm
+
+end FirstOrder
