Logic/Predicate/Meta.lean
@@ -1,68 +1,63 @@
 import Logic.Predicate.Coding
+import Logic.Predicate.Elab
 import Logic.Vorspiel.Meta
 open Qq Lean Elab Meta Tactic
 
 -- SubTerm normalization
+
+namespace FirstOrder
+
 namespace SubTerm
 
 namespace Meta
 
 section lemmata
-variable {L : Language.{u}} {μ : Type v} {n}
+variable {L : ℕ → Type u} {μ : Type v} {n}
+
+section Hom
+
+variable (ω : Hom L μ₁ n₁ μ₂ n₂)
+
+lemma hom_func_eq_of_eq {k} (f : L k) {v : Fin k → SubTerm L μ₁ n₁} {v'} (h : ω ∘ v = v') :
+    ω (func f v) = func f v' :=
+  by simp[Hom.func, Function.comp, ←h]
+
+lemma hom_finitary_eq_of_eq {k} (f : Finitary L k) {v : Fin k → SubTerm L μ₁ n₁} {v'} (h : ω ∘ v = v') :
+    ω (f.operator v) = f.operator v' :=
+  by simp[Hom.operator, Function.comp, ←h]
+
+end Hom
 
 section substs
 
-lemma substs_bvar_of_eq {n n'} {w : Fin n → SubTerm L μ n'} {x : Fin n} {t} (h : w x = t) :
+lemma substs_bvar_eq_of_eq {n n'} {w : Fin n → SubTerm L μ n'} {x : Fin n} {t} (h : w x = t) :
     substs w #x = t :=
   by simp[h]
 
-lemma substs_func_of_eq {n n'} {w : Fin n → SubTerm L μ n'} {k} (f : L.func k) {v : Fin k → SubTerm L μ n} {v'} (h : substs w ∘ v = v') :
-    substs w (func f v) = func f v' :=
-  by simp[substs_func, Function.comp, ←h]
-
-lemma substs_substs_of_eq {l k n} {v : Fin l → SubTerm L μ k} {w : Fin k → SubTerm L μ n}
-  {t : SubTerm L μ l} {v'} {t'}
+lemma substs_substs_eq_of_eq {l k n} {v : Fin l → SubTerm L μ k} {w : Fin k → SubTerm L μ n} {t : SubTerm L μ l} {v'} {t'}
   (hv : substs w ∘ v = v') (ht : substs v' t = t') :
     substs w (substs v t) = t' := by simp[substs_substs, ←hv, ←ht]
 
-lemma substs_eq_of_eq {k n} {w w' : Fin k → SubTerm L μ n} {t t' : SubTerm L μ k} {u}
+lemma substs_eq_eq_of_eq {k n} {w w' : Fin k → SubTerm L μ n} {t t' : SubTerm L μ k} {u}
   (hw : w = w') (ht : t = t') (h : substs w' t' = u) : substs w t = u := hw ▸ ht ▸ h
-
-lemma substs_finitary_of_eq {n n'} {w : Fin n → SubTerm L μ n'} {k} (f : Finitary L k) {v : Fin k → SubTerm L μ n} {v'} (h : substs w ∘ v = v') :
-    substs w (f.operator v) = f.operator v' :=
-  by simp[Operator.substs_operator, Function.comp, ←h]
 
 end substs
 
 section shift
 
-lemma shift_func_of_eq {n} (f : L.func k) {v : Fin k → SyntacticSubTerm L n} {v'} (h : shift ∘ v = v') :
-    shift (func f v) = func f v' :=
-  by simp[shift_func, Function.comp, ←h]
-
-lemma shift_substs_of_eq {t : SyntacticSubTerm L k} {w : Fin k → SyntacticSubTerm L n} {t' t'' w'}
+lemma shift_substs_eq_of_eq {t : SyntacticSubTerm L k} {w : Fin k → SyntacticSubTerm L n} {t' t'' w'}
   (ht : shift t = t') (hw : shift ∘ w = w') (ht' : substs w' t' = t'') :
     shift (substs w t) = t'' := by
   simp[←ht, ←hw, ←ht', shift, substs, map, bind_bind]
-
-lemma shift_finitary_of_eq {n} (f : Finitary L k) {v : Fin k → SyntacticSubTerm L n} {v'} (h : shift ∘ v = v') :
-    shift (f.operator v) = f.operator v' :=
-  by simp[Operator.shift_operator, Function.comp, ←h]
 
 end shift
 
 section bShift
 
-lemma bShift_func_of_eq (f : L.func k) {v : Fin k → SubTerm L μ n} {v'} (h : bShift ∘ v = v'):
-    bShift (func f v) = func f v' := by simp[←h, bShift_func]; funext x; simp
-
-lemma bShift_substs_of_eq {w : Fin k → SubTerm L μ n} {t : SubTerm L μ k} {w' t'}
+lemma bShift_substs_eq_of_eq {w : Fin k → SubTerm L μ n} {t : SubTerm L μ k} {w' t'}
   (hw : bShift ∘ w = w') (ht : substs w' t = t') :
     bShift (substs w t) = t' := by
   simp[←hw, ←ht, bShift, substs, map, bind_bind]; congr
-
-lemma bShift_finitary_of_eq (f : Finitary L k) {v : Fin k → SubTerm L μ n} {v'} (h : bShift ∘ v = v'):
-    bShift (f.operator v) = f.operator v' := by simp[←h, Operator.bShift_operator f v, Function.comp]
 
 end bShift
 
@@ -74,18 +69,10 @@ lemma free_bvar_last (n : ℕ) : free (#⟨n, Nat.lt.base n⟩ : SyntacticSubTer
 lemma free_bvar_of_lt (x : Fin (n + 1)) (h : x.val < n) : free (#x : SyntacticSubTerm L (n + 1)) = #⟨x, h⟩ :=
   free_bvar_castSucc (L := L) ⟨x, h⟩
 
-lemma free_func_of_eq {n} (f : L.func k) {v : Fin k → SyntacticSubTerm L (n + 1)} {v'} (h : free ∘ v = v') :
-    free (func f v) = func f v' :=
-  by simp[free_func, Function.comp, ←h]
-
-lemma free_substs_of_eq {t : SyntacticSubTerm L k} {w : Fin k → SyntacticSubTerm L (n + 1)} {t' w' t''}
+lemma free_substs_eq_of_eq {t : SyntacticSubTerm L k} {w : Fin k → SyntacticSubTerm L (n + 1)} {t' w' t''}
   (ht : shift t = t') (hw : free ∘ w = w') (ht' : substs w' t' = t'') :
     free (substs w t) = t'' := by
   simp[←ht, ←hw, ←ht', shift, map, free, substs, bind_bind]
-
-lemma free_finitary_of_eq {n} (f : Finitary L k) {v : Fin k → SyntacticSubTerm L (n + 1)} {v'} (h : free ∘ v = v') :
-    free (f.operator v) = f.operator v' :=
-  by simp[Operator.free_operator, Function.comp, ←h]
 
 end free
 
@@ -100,23 +87,15 @@ lemma fix_bvar_zero (n : ℕ) : fix &0 = (#⟨n, Nat.lt.base n⟩ : SyntacticSub
 lemma fix_bvar_succ (x) (n : ℕ) : fix (&(x + 1) : SyntacticSubTerm L (n + 1)) = &x :=
   SubTerm.fix_fvar_succ x
 
-lemma fix_func_of_eq {n} (f : L.func k) {v : Fin k → SyntacticSubTerm L n} {v'} (h : fix ∘ v = v') :
-    fix (func f v) = func f v' :=
-  by simp[fix_func, Function.comp, ←h]
-
-lemma fix_substs_of_eq {k} {t : SyntacticSubTerm L k} {w : Fin k → SyntacticSubTerm L n} {t' t'' w' w'' i}
+lemma fix_substs_eq_of_eq {k} {t : SyntacticSubTerm L k} {w : Fin k → SyntacticSubTerm L n} {t' t'' w' w'' i}
   (ht : fix t = t') (hw : fix ∘ w = w') (hi : Fin.last n = i) (hw' : w' <: #i = w'') (ht' : substs w'' t' = t''):
     fix (substs w t) = t'' := by
   simp[←ht, ←hw, ←hi, ←hw', ←ht', shift, map, fix, substs, bind_bind, Function.comp]; congr
   · funext x; cases x <;> simp
 
-lemma fix_finitary_of_eq {n} (f : Finitary L k) {v : Fin k → SyntacticSubTerm L n} {v'} (h : fix ∘ v = v') :
-    fix (f.operator v) = f.operator v' :=
-  by simp[Operator.fix_operator, Function.comp, ←h]
-
 end fix
 
-lemma func_congr  {k} (f : L.func k) {v₁ v₂ : Fin k → SyntacticSubTerm L n} (h : v₁ = v₂):
+lemma func_congr  {k} (f : L k) {v₁ v₂ : Fin k → SyntacticSubTerm L n} (h : v₁ = v₂):
     func f v₁ = func f v₂ := by simp[←h]
 
 lemma finitary_congr  {k} (f : Finitary L k) {v₁ v₂ : Fin k → SyntacticSubTerm L n} (h : v₁ = v₂):
@@ -131,7 +110,7 @@ lemma shift_congr_eq {t t' : SyntacticSubTerm L n} {u} (e : t = t') (h : shift t
 lemma bShift_congr_eq {t t' : SubTerm L μ n} {u} (e : t = t') (h : bShift t' = u) :
   bShift t = u := Eq.trans (congr_arg _ e) h
 
-section
+section Const
 variable (c : Const L)
 
 @[simp] lemma free_const :
@@ -154,54 +133,41 @@ variable (c : Const L)
     bShift (c : SubTerm L μ n) = c :=
   by simp[bShift]
 
-variable [L.Zero] [L.One] [L.Add]
+variable [Language.Zero L] [Language.One L] [Language.Add L]
 
-lemma natLit_succ_of_eq {z : ℕ} (t : SubTerm L μ n) (h : natLit L z.succ = t) :
+lemma natLit_succ_eq_of_eq {z : ℕ} (t : SubTerm L μ n) (h : natLit L z.succ = t) :
   natLit L z.succ.succ = func Language.Add.add ![t, func Language.One.one ![]] := by rw[←h]; rfl
 
-end
-
-lemma eq_substs_zero_of_eq {s t : Term L μ} (h : s = t) : s = substs ![t] #0 := by simp[h]
-
-lemma const_eq_substs_sonst_of_eq (c : Const L) {s : Term L μ} : c.const = substs ![s] c.const := by simp
-
-lemma eq_substs_func_of_eq {k} {s : Term L μ} (f : L.func k) {v : Fin k → Term L μ} {v' : Fin k → SubTerm L μ 1}
-  (h : ∀ i, v i = substs ![s] (v' i)) : func f v = substs ![s] (func f v') := by simp[substs_func, ←h]
-
-lemma eq_substs_substs_of_eq {k} {s : Term L μ} (t : SubTerm L μ k) {v : Fin k → Term L μ} {v' : Fin k → SubTerm L μ 1}
-  (h : ∀ i, v i = substs ![s] (v' i)) : substs v t = substs ![s] (substs v' t) := by simp[substs_substs, Function.comp, ←h]
-
-lemma eq_substs_substs_nil (v) (s : Term L μ) {t : Term L μ} {t'} (ht : substs v t = t') :
-  t = substs ![s] t' := by simp[←ht, substs_substs]
+end Const
 
 end lemmata
 
-partial def resultSubsts {L : Q(Language.{u})} {k n : Q(ℕ)} (w : Q(Fin $k → SyntacticSubTerm $L $n)) :
+partial def resultSubsts {L : Q(ℕ → Type u)} {k n : Q(ℕ)} (w : Q(Fin $k → SyntacticSubTerm $L $n)) :
     (t : Q(SyntacticSubTerm $L $k)) → MetaM ((res : Q(SyntacticSubTerm $L $n)) × Q(substs $w $t = $res))
   | ~q(#$x)                          => do
     let ⟨t, ht⟩ ← vectorQNth (u := u) k w x
-    return ⟨t, q(substs_bvar_of_eq $ht)⟩
+    return ⟨t, q(substs_bvar_eq_of_eq $ht)⟩
   | ~q(&$x)                          => pure ⟨q(&$x), q(substs_fvar $w $x)⟩
   | ~q(func (arity := $arity) $f $v) => do
     let ⟨v', ve⟩ ← resultVectorOfResultFun (u := u) (v := u)
       (α := q(SyntacticSubTerm $L $k)) (β := q(SyntacticSubTerm $L $n))
       q(substs $w) (resultSubsts w) arity v
-    return ⟨q(func $f $v'), q(substs_func_of_eq $f $ve)⟩
+    return ⟨q(func $f $v'), q(hom_func_eq_of_eq _ $f $ve)⟩
   | ~q(Operator.const $c)            => pure ⟨q(Operator.const $c), q(substs_const $c)⟩
   | ~q(Operator.operator (ι := Fin $arity) $f $v) => do
     let ⟨v', ve⟩ ← resultVectorOfResultFun (u := u) (v := u)
       (α := q(SyntacticSubTerm $L $k)) (β := q(SyntacticSubTerm $L $n))
       q(substs $w) (resultSubsts w) arity v
-    return ⟨q(Operator.operator $f $v'), q(substs_finitary_of_eq $f $ve)⟩
+    return ⟨q(Operator.operator $f $v'), q(hom_finitary_eq_of_eq _ $f $ve)⟩
   | ~q(substs (n := $l) $v $t)       => do
     let ⟨v', ve⟩ ← resultVectorOfResultFun (u := u) (v := u)
       (α := q(SyntacticSubTerm $L $k)) (β := q(SyntacticSubTerm $L $n))
       q(@SubTerm.substs $L ℕ $k $n $w) (resultSubsts w) l v
     let ⟨p', pe⟩ ← resultSubsts v' t
-    return ⟨p', q(substs_substs_of_eq $ve $pe)⟩
+    return ⟨p', q(substs_substs_eq_of_eq $ve $pe)⟩
   | ~q($t)                           => pure ⟨q(substs $w $t), q(rfl)⟩
 
-partial def resultShift {L : Q(Language.{u})} {n : Q(ℕ)} : (t : Q(SyntacticSubTerm $L $n)) →
+partial def resultShift {L : Q(ℕ → Type u)} {n : Q(ℕ)} : (t : Q(SyntacticSubTerm $L $n)) →
     MetaM ((res : Q(SyntacticSubTerm $L $n)) × Q(SubTerm.shift $t = $res))
   | ~q(#$x)                          => pure ⟨q(#$x), q(SubTerm.shift_bvar $x)⟩
   | ~q(&$x)                          =>  do
@@ -212,24 +178,24 @@ partial def resultShift {L : Q(Language.{u})} {n : Q(ℕ)} : (t : Q(SyntacticSub
     let ⟨v', ve'⟩ ← resultVectorOfResultFun (u := u) (v := u)
       (α := q(SyntacticSubTerm $L $n)) (β := q(SyntacticSubTerm $L $n))
       q(@shift $L $n) resultShift arity v
-    return ⟨q(func $f $v'), q(shift_func_of_eq $f $ve')⟩
+    return ⟨q(func $f $v'), q(hom_func_eq_of_eq _ $f $ve')⟩
   | ~q(substs (n := $k) $w $t)       => do
     let ⟨t', te⟩ ← resultShift (L := L) (n := k) t
     let ⟨w', we⟩ ← resultVectorOfResultFun (u := u) (v := u)
       (α := q(SyntacticSubTerm $L $n)) (β := q(SyntacticSubTerm $L $n))
       q(@SubTerm.shift $L $n) resultShift k w
     let ⟨t'', t'e⟩ ← resultSubsts w' t'
-    return ⟨t'', q(shift_substs_of_eq $te $we $t'e)⟩
+    return ⟨t'', q(shift_substs_eq_of_eq $te $we $t'e)⟩
   | ~q(SubTerm.Operator.const $c)    => pure ⟨q(SubTerm.Operator.const $c), q(shift_const $c)⟩
   | ~q(Operator.operator (ι := Fin $arity) $f $v) => do
     let ⟨v', ve'⟩ ← resultVectorOfResultFun (u := u) (v := u)
       (α := q(SyntacticSubTerm $L $n)) (β := q(SyntacticSubTerm $L $n))
       q(@shift $L $n) resultShift arity v
-    return ⟨q(Operator.operator $f $v'), q(shift_finitary_of_eq $f $ve')⟩
+    return ⟨q(Operator.operator $f $v'), q(hom_finitary_eq_of_eq _ $f $ve')⟩
   | ~q($t)                           => do
     return ⟨q(shift $t), q(rfl)⟩
 
-partial def resultFree {L : Q(Language.{u})} {n : Q(ℕ)} : (t : Q(SyntacticSubTerm $L ($n + 1))) →
+partial def resultFree {L : Q(ℕ → Type u)} {n : Q(ℕ)} : (t : Q(SyntacticSubTerm $L ($n + 1))) →
     MetaM ((res : Q(SyntacticSubTerm $L $n)) × Q(SubTerm.free $t = $res))
   | ~q(#$x)                                       => do
     let n ←whnf n 
@@ -251,26 +217,24 @@ partial def resultFree {L : Q(Language.{u})} {n : Q(ℕ)} : (t : Q(SyntacticSubT
     let ⟨v', ve'⟩ ← resultVectorOfResultFun (u := u) (v := u)
       (α := q(SyntacticSubTerm $L ($n + 1))) (β := q(SyntacticSubTerm $L $n))
       q(@free $L $n) resultFree arity v
-    return ⟨q(func $f $v'), q(free_func_of_eq $f $ve')⟩
+    return ⟨q(func $f $v'), q(hom_func_eq_of_eq _ $f $ve')⟩
   | ~q(substs (n := $k) $w $t)                    => do
     let ⟨t', te⟩ ← resultShift (L := L) (n := k) t
     let ⟨w', we⟩ ← resultVectorOfResultFun (u := u) (v := u)
       (α := q(SyntacticSubTerm $L ($n + 1))) (β := q(SyntacticSubTerm $L $n))
       q(@SubTerm.free $L $n) resultFree k w
     let ⟨t'', t'e⟩ ← resultSubsts w' t'
-    return ⟨t'', q(free_substs_of_eq $te $we $t'e)⟩
+    return ⟨t'', q(free_substs_eq_of_eq $te $we $t'e)⟩
   | ~q(SubTerm.Operator.const $c)                 => return ⟨q(SubTerm.Operator.const $c), q(free_const _)⟩
   | ~q(Operator.operator (ι := Fin $arity) $f $v) => do
     let ⟨v', ve'⟩ ← resultVectorOfResultFun (u := u) (v := u)
       (α := q(SyntacticSubTerm $L ($n + 1))) (β := q(SyntacticSubTerm $L $n))
       q(@free $L $n) resultFree arity v
-    return ⟨q(Operator.operator $f $v'), q(free_finitary_of_eq $f $ve')⟩
+    return ⟨q(Operator.operator $f $v'), q(hom_finitary_eq_of_eq _ $f $ve')⟩
   | ~q($t)                                        => do
     return ⟨q(SubTerm.free $t), q(rfl)⟩
 
-#check fix_substs_of_eq
-
-partial def resultFix {L : Q(Language.{u})} {n : Q(ℕ)} : (t : Q(SyntacticSubTerm $L $n)) →
+partial def resultFix {L : Q(ℕ → Type u)} {n : Q(ℕ)} : (t : Q(SyntacticSubTerm $L $n)) →
     MetaM ((res : Q(SyntacticSubTerm $L ($n + 1))) × Q(SubTerm.fix $t = $res))
   | ~q(#$x)                                       => do
     let some xval := (← finQVal (n := q(.succ $n)) x) | throwError f!"Fail: FinQVal {x}"
@@ -289,7 +253,7 @@ partial def resultFix {L : Q(Language.{u})} {n : Q(ℕ)} : (t : Q(SyntacticSubTe
     let ⟨v', ve'⟩ ← resultVectorOfResultFun (u := u) (v := u)
       (α := q(SyntacticSubTerm $L $n)) (β := q(SyntacticSubTerm $L ($n + 1)))
       q(@fix $L $n) resultFix arity v
-    return ⟨q(func $f $v'), q(fix_func_of_eq $f $ve')⟩
+    return ⟨q(func $f $v'), q(hom_func_eq_of_eq _ $f $ve')⟩
   | ~q(substs (n := $k) $w $t)                    => do
     let ⟨t', ht⟩ ← resultFix (L := L) (n := k) t
     let ⟨w', hw⟩ ← resultVectorOfResultFun (u := u) (v := u)
@@ -300,18 +264,18 @@ partial def resultFix {L : Q(Language.{u})} {n : Q(ℕ)} : (t : Q(SyntacticSubTe
     let hz : Q(Fin.last $n = $z) := (q(@rfl (Fin ($n + 1)) $z) : Expr)
     let ⟨w'', hw'⟩ ← vectorAppend k w' q(#$z)
     let ⟨t'', ht'⟩ ← resultSubsts w'' t'
-    return ⟨t'', q(fix_substs_of_eq $ht $hw $hz $hw' $ht')⟩
+    return ⟨t'', q(fix_substs_eq_of_eq $ht $hw $hz $hw' $ht')⟩
   | ~q(SubTerm.Operator.const $c)                 => return ⟨q(SubTerm.Operator.const $c), q(fix_const _)⟩
   | ~q(Operator.operator (ι := Fin $arity) $f $v) => do
     let ⟨v', ve'⟩ ← resultVectorOfResultFun (u := u) (v := u)
       (α := q(SyntacticSubTerm $L $n)) (β := q(SyntacticSubTerm $L ($n + 1)))
       q(@fix $L $n) resultFix arity v
-    return ⟨q(Operator.operator $f $v'), q(fix_finitary_of_eq $f $ve')⟩
+    return ⟨q(Operator.operator $f $v'), q(hom_finitary_eq_of_eq _ $f $ve')⟩
   | ~q($t)                                        => do
     return ⟨q(SubTerm.fix $t), q(rfl)⟩
 
 elab "dbgResultFix" : term => do
-  let L : Q(Language.{0}) := q(Language.oRing)
+  let L : Q(ℕ → Type) := q(Language.ORingFunc)
   let t : Q(SyntacticTerm $L) := q(ᵀ“((&2 + 1) + 9) * (#0 + 1)ᵀ⟦&2 + 1, 6⟧ ”)
   let ⟨e, eq⟩ ← resultFix (L := L) (n := q(0)) t
   logInfo m! "{t}\n ⟹\n {e}"
@@ -320,7 +284,7 @@ elab "dbgResultFix" : term => do
 
 #eval dbgResultFix
 
-partial def resultBShift {L : Q(Language.{u})} {n : Q(ℕ)} : (t : Q(SyntacticSubTerm $L $n)) →
+partial def resultBShift {L : Q(ℕ → Type u)} {n : Q(ℕ)} : (t : Q(SyntacticSubTerm $L $n)) →
     MetaM ((res : Q(SyntacticSubTerm $L ($n + 1))) × Q(bShift $t = $res))
   | ~q(#$x)                                       => do
     let some xval := (← finQVal (n := q(.succ $n)) x) | throwError f!"Fail: FinQVal {x}"
@@ -332,19 +296,19 @@ partial def resultBShift {L : Q(Language.{u})} {n : Q(ℕ)} : (t : Q(SyntacticSu
     let ⟨v', ve'⟩ ← resultVectorOfResultFun (u := u) (v := u)
       (α := q(SyntacticSubTerm $L $n)) (β := q(SyntacticSubTerm $L ($n + 1)))
       q(@bShift $L ℕ $n) resultBShift arity v
-    return ⟨q(func $f $v'), q(bShift_func_of_eq $f $ve')⟩
+    return ⟨q(func $f $v'), q(hom_func_eq_of_eq _ $f $ve')⟩
   | ~q(substs (n := $k) $w $t)                    => do
     let ⟨w', we⟩ ← resultVectorOfResultFun (u := u) (v := u)
       (α := q(SyntacticSubTerm $L $n)) (β := q(SyntacticSubTerm $L ($n + 1)))
       q(@SubTerm.bShift $L ℕ $n) resultBShift k w
     let ⟨t', te⟩ ← resultSubsts w' t
-    return ⟨t', q(bShift_substs_of_eq $we $te)⟩
+    return ⟨t', q(bShift_substs_eq_of_eq $we $te)⟩
   | ~q(SubTerm.Operator.const $c)                 => return ⟨q(SubTerm.Operator.const $c), q(bShift_const $c)⟩
   | ~q(Operator.operator (ι := Fin $arity) $f $v) => do
     let ⟨v', ve'⟩ ← resultVectorOfResultFun (u := u) (v := u)
       (α := q(SyntacticSubTerm $L $n)) (β := q(SyntacticSubTerm $L ($n + 1)))
       q(@bShift $L ℕ $n) resultBShift arity v
-    return ⟨q(Operator.operator $f $v'), q(bShift_finitary_of_eq $f $ve')⟩
+    return ⟨q(Operator.operator $f $v'), q(hom_finitary_eq_of_eq _ $f $ve')⟩
   | ~q($t)                                        => do
     return ⟨q(bShift $t), q(rfl)⟩
 
@@ -353,7 +317,7 @@ inductive NumeralUnfoldOption
   | unfoldSucc
   | all
 
-partial def natLitResult {L : Q(Language.{u})}
+partial def natLitResult {L : Q(ℕ → Type u)}
   (iz : Q(Language.Zero $L)) (io : Q(Language.One $L)) (ia : Q(Language.Add $L)) (n : Q(ℕ)) :
     NumeralUnfoldOption → (z : Q(ℕ)) → MetaM $ (res : Q(SyntacticSubTerm $L $n)) × Q(natLit $L $z = $res)
   | NumeralUnfoldOption.none       =>
@@ -376,10 +340,10 @@ partial def natLitResult {L : Q(Language.{u})}
       | ~q(1)      => return ⟨q(natLit $L 1), q(rfl)⟩
       | ~q(.succ $ .succ $z) => do
         let ⟨e, he⟩ ← natLitResult iz io ia n NumeralUnfoldOption.all q(.succ $z)
-        return ⟨q(func Language.Add.add ![$e, natLit $L 1]), q(natLit_succ_of_eq $e $he)⟩
+        return ⟨q(func Language.Add.add ![$e, natLit $L 1]), q(natLit_succ_eq_of_eq $e $he)⟩
       | ~q($z)      => return ⟨q(natLit $L $z), q(rfl)⟩
 
-partial def result (tp : NumeralUnfoldOption) {L : Q(Language.{u})} {n : Q(ℕ)} : (t : Q(SyntacticSubTerm $L $n)) →
+partial def result (tp : NumeralUnfoldOption) {L : Q(ℕ → Type u)} {n : Q(ℕ)} : (t : Q(SyntacticSubTerm $L $n)) →
     MetaM ((res : Q(SyntacticSubTerm $L $n)) × Q($t = $res))
   | ~q(#$x)                                       => pure ⟨q(#$x), q(rfl)⟩
   | ~q(&$x)                                       => pure ⟨q(&$x), q(rfl)⟩
@@ -394,7 +358,7 @@ partial def result (tp : NumeralUnfoldOption) {L : Q(Language.{u})} {n : Q(ℕ)}
     let ⟨t', te⟩ ← result tp (L := L) (n := k) t
     let ⟨w', we⟩ ← resultVectorOfResult (α := q(SyntacticSubTerm $L $n)) (u := u) (result tp) k w
     let ⟨e, t''⟩ ← resultSubsts (u := u) w' t'
-    return ⟨e, q(substs_eq_of_eq $we $te $t'')⟩
+    return ⟨e, q(substs_eq_eq_of_eq $we $te $t'')⟩
   | ~q(shift $t)                                  => do
     let ⟨t', te⟩ ← result tp (L := L) (n := q($n)) t
     let ⟨t'', tee⟩ ← resultShift (L := L) (n := n) t'
@@ -419,11 +383,11 @@ elab "dbg" : tactic => do
   let c : Q(DbgResult (SyntacticSubTerm $L $n) $t) := (q(DbgResult.intro ($t) $tn $e) : Expr)
   Lean.Elab.Tactic.closeMainGoal c
 
-example {t : SyntacticSubTerm Language.oRing 2} : DbgResult (SyntacticSubTerm Language.oRing 12)
+example {t : SyntacticSubTerm Language.ORingFunc 2} : DbgResult (SyntacticSubTerm Language.ORingFunc 12)
     (shift $ substs ![substs ![ᵀ“6”, ᵀ“&7”] t, ᵀ“3 + &6”] ᵀ“(ᵀ!t) + (#0 * ᵀ!(shift ᵀ“#1 + 9 * #1”)) + &7”) :=
   by dbg
 
-example (t : SyntacticSubTerm Language.oRing 3) : DbgResult (SyntacticSubTerm Language.oRing 12)
+example (t : SyntacticSubTerm Language.ORingFunc 3) : DbgResult (SyntacticSubTerm Language.ORingFunc 12)
     $ free $ ᵀ“((#0 + #1 + #2 + 8 * ᵀ!t) ᵀ⟦#2, 7, 4⟧ ᵀ⟦4, 4, 5⟧) * 8” :=
   by dbg
 
@@ -432,3 +396,5 @@ example : 1 ≠ 2 := of_decide_eq_true rfl
 end Meta
 
 end SubTerm
+
+end FirstOrder
